pulse/lib/steel/pulse/Pulse.Checker.Inference.fsti
@@ -8,6 +8,8 @@ module R = FStar.Reflection
 
 val uvar_id : eqtype
 
+val uvar_id_to_string (_:uvar_id) : string
+
 val is_uvar (t:term) : option uvar_id
 
 val gen_uvar (_:unit) : T.Tac (r:(uvar_id & term){Some? (is_uvar (snd r)) /\
@@ -19,6 +21,9 @@ val try_inst_uvs_in_goal (ctxt:term)
 
 val infer (head:term) (t_head:term) (ctxt_pre:term) (r:range)
   : T.Tac st_term
+
+val solutions_to_string (sol:list (uvar_id & term))
+  : T.Tac string
 
 val apply_solution (sol:list (uvar_id & term)) (t:term)
   : term
